backend/XTL.ml
@@ -125,10 +125,10 @@ let rec set_vars_type vl tyl =
 let unify_var_type v1 v2 =
   if typeof v1 <> typeof v2 then raise Type_error
 
-let type_annot_arg a ty =
+let rec type_annot_arg a ty =
   match a with
   | AA_base v -> set_var_type v ty
-  | AA_longofwords(v1, v2) -> set_var_type v1 Tint; set_var_type v2 Tint
+  | AA_longofwords(a1, a2) -> type_annot_arg a1 Tint; type_annot_arg a2 Tint
   | _ -> ()
 
 let type_instr = function
